ODerivations.v
@@ -1,4 +1,4 @@
-Require Import Defs Debruijn Occurrences Address.
+Require Import Utils Defs Debruijn Occurrences Address.
 Require Import StringUtils Datatypes.
 Require DecimalString.
 Import ListNotations.
@@ -19,6 +19,7 @@ Fixpoint subderiv (d:oderivation)(a:address): option oderivation :=
   | _, _ => None
   end.
 
+Definition is_subderiv (d1 d2: oderivation): Prop := exists a, subderiv d2 a = Some d1. 
 Local Open Scope string_scope.
 
 Definition Subderiv_example: oderivation := 
@@ -90,13 +91,36 @@ Instance ls_eqb : Eqb (nat*osequent) :=
   fix ls_eqb ls1 ls2 :=
     let (n1, s1) := ls1 in (let (n2, s2) := ls2 in (n1 =? n2) && (s1 =? s2)).
 
+Lemma list_assoc_get_Some : forall n l s, list_assoc n l = Some s -> get n l = s.
+Proof.
+  intros; induction l.
+  -- inversion H.
+  -- simpl in *; destruct a; destruct (n=?n0).
+    + injection H as H; subst; trivial.
+    + apply IHl; assumption.
+Qed.
+
+Lemma list_assoc_get_None : forall n l, list_assoc n l = None -> get n l = (⊢ []).
+Proof.
+  intros; induction l; intros; simpl in *; trivial; destruct a; destruct (n =? n0); 
+  try discriminate H; apply IHl; assumption.
+Qed.
+
+Instance : EqbSpec (nat*osequent).
+Proof.
+  red.
+  destruct x; destruct y; cbn. 
+  case eqbspec; [ intros <- | cons ]; case eqbspec; [ intros <- | cons ]; simpl.
+  constructor; trivial.
+Qed.
+
 (* Boolean version of valid inference structure for one step *)
 
 Definition ovalid_deriv_step '(ORule ls R s ld) :=
   match ls, R, s, List.map oclaim ld, List.map backedges ld with
   | ls1, Ax, (⊢ A::A'::Γ ), [], _                => equivb A' (occ_dual A)
-  | _, TopR,  (⊢ {⊤, _}::Γ ), _, _           => true 
-  | _, OneR,  (⊢ [{! ,_}]), _, _               => true
+  | _, TopR,  (⊢ {⊤, _}::Γ ), [], _           => true 
+  | _, OneR,  (⊢ [{! ,_}]), [], _               => true
   | ls1, BotR,  (⊢ {⊥, _}::Γ), [s], [ls2]  => (s =? (⊢ Γ)) 
                                                                        &&& 
                                                                   ((ls2 =? (lift ls1)) ||| (ls2 =? (1, s):: (lift ls1)))
@@ -120,36 +144,36 @@ Definition ovalid_deriv_step '(ORule ls R s ld) :=
                                                           => (F =? F') &&& (G =? G') 
                                                                               &&& (a1 =? l::a) &&& (a2 =? r::a) 
                                                                               &&& (Γ1 =? Γ) &&& (Γ2 =? Γ) 
-                                                                              &&& ((ls2 =? (lift ls1)) ||| (ls2 =? ((1, s) :: (lift ls1))))
-                                                                              &&& ((ls3 =? (lift ls1)) ||| (ls3 =? ((1, s) :: (lift ls1))))
+                                                                              &&& ((ls2 =? (lift ls1)) ||| (ls2 =? ((0, s) :: (lift ls1))))
+                                                                              &&& ((ls3 =? (lift ls1)) ||| (ls3 =? ((0, s) :: (lift ls1))))
 
   | ls1, And_mult,  (⊢ { F⊗G, a }::Γ), [(⊢ {F',a1}::Γ1);(⊢ {G',a2}::Γ2)], [ls2;ls3]
                                                           => (F =? F') &&& (G =? G') 
                                                                               &&& (a1 =? l::a) &&& (a2 =? r::a) 
                                                                               &&& ((app Γ1 Γ2) =? Γ) 
-                                                                              &&& ((ls2 =? (lift ls1)) ||| (ls2 =? ((1, s) :: (lift ls1))))
-                                                                              &&& ((ls3 =? (lift ls1)) ||| (ls3 =? ((1, s) :: (lift ls1))))
+                                                                              &&& ((ls2 =? (lift ls1)) ||| (ls2 =? ((0, s) :: (lift ls1))))
+                                                                              &&& ((ls3 =? (lift ls1)) ||| (ls3 =? ((0, s) :: (lift ls1))))
 
   | ls1, Cut,   (⊢  Γ), [(⊢ A:: Γ1);(⊢ B:: Γ2)], [ls2;ls3]
                                                           => ( Γ =? Γ1 ++  Γ2 ) &&& (B =? (occ_dual A))  
                                                                                             &&& disjoint_addr_listb (occ_addr A)(ocontext_addr Γ1)
                                                                                             &&& disjoint_addr_listb (occ_addr B)(ocontext_addr Γ2)
-                                                                                            &&& ((ls2 =? (lift ls1)) ||| (ls2 =? ((1,s) :: (lift ls1))))
-                                                                                            &&& ((ls3 =? (lift ls1)) ||| (ls3 =? ((1,s) :: (lift ls1))))
+                                                                                            &&& (((ls2 =? (lift ls1)) &&& (ls3 =? (lift ls1))) |||
+                                                                                            (((ls2 =? ((0, s) :: (lift ls1))) &&& (ls3 =? ((0, s) :: (lift ls1))))))
 
   | ls1, Ex,  (⊢ Γ), [(⊢Γ')], [ls2]         => (list_permut Γ Γ') 
                                                                       &&& 
-                                                              ((ls2 =? (lift ls1)) ||| (ls2 =? ((1, s) :: (lift ls1))))
+                                                              ((ls2 =? (lift ls1)) ||| (ls2 =? ((0, s) :: (lift ls1))))
 
   | ls1, Mu, (⊢ { µ F, a }::Γ), [(⊢{G,a'}::Γ')], [ls2] 
                                                         => (G =? (F[[ %0 := µ F ]]) ) &&& (Γ =? Γ') &&& (a' =? i::a)
                                                                                         &&& 
-                                                             ((ls2 =? (lift ls1)) ||| (ls2 =? (1, s) :: (lift ls1)))
+                                                             ((ls2 =? (lift ls1)) ||| (ls2 =? (0, s) :: (lift ls1)))
 
   | ls1, Nu, (⊢ { ν F, a }::Γ), [(⊢{G,a'}::Γ')], [ls2] 
                                                        => (G =? (F[[ %0 := ν F ]])) &&& (Γ =? Γ') &&& (a' =? i::a)
                                                                                         &&& 
-                                                            ((ls2 =? (lift ls1)) ||| (ls2 =? (1, s) :: (lift ls1)))
+                                                            ((ls2 =? (lift ls1)) ||| (ls2 =? (0, s) :: (lift ls1)))
 
   | ls, BackEdge n, s, [], _ => match list_assoc n ls with
                                                 | None => false
@@ -178,6 +202,12 @@ Proof.
  apply IH'.
 Qed.
 
+Lemma oderivation_ind'' (P: oderivation -> Prop) :
+  (forall d d', is_subderiv d' d -> d <> d' -> P d') ->
+  forall d, P d.
+Proof.
+Admitted.
+  
 Local Open Scope string_scope.
 
 Definition oderiv_example :=
@@ -219,6 +249,24 @@ Fixpoint count_occ' (l : list Occurrence) (x : formula) : nat :=
   | { y, a } :: l' => if (x =? y) then 1 + (count_occ' l' x) else (count_occ' l' x)
   end.
 
+Local Open Scope list_scope.
+
+Lemma count_occ'_app :  forall l1 l2 f, count_occ' (l1 ++ l2) f = count_occ' l1 f + count_occ' l2 f.
+Proof.
+  induction l1; intros; simpl in *; trivial.
+  destruct a; destruct (f =? F); trivial.
+  rewrite plus_Sn_m; rewrite IHl1; trivial.
+Qed.
+
+Lemma count_occ'_permut : forall o1 o2 l1 l2 f, 
+                                        count_occ' (l1 ++ o1 :: o2 :: l2) f = count_occ' (l1 ++ o2 :: o1 :: l2) f.
+Proof.
+  intros.
+  destruct o1; destruct o2.
+  rewrite count_occ'_app, count_occ'_app; simpl; destruct (f =? F); destruct (f =? F0); trivial.
+Qed.
+
+
 Local Open Scope nat_scope.
  
 Inductive OValid : oderivation -> Prop :=
@@ -259,7 +307,7 @@ Inductive OValid : oderivation -> Prop :=
                             -> OValid (ORule ls And_mult (⊢ { F⊗G, a } :: (app Γ1 Γ2)) [d1;d2])
  | V_Cut d1 d2 A Γ1 Γ2 ls a1 a2 :
                             OValid d1 -> OValid d2 
-                            -> OClaim d1 (⊢ { dual A, a1}::Γ1) -> OClaim d2 (⊢ { A, a2 }::Γ2) 
+                            -> OClaim d1 (⊢ { A, a1}::Γ1) -> OClaim d2 (⊢ { dual A, a2 }::Γ2) 
                             -> disjoint_addr_list a1 (ocontext_addr Γ1) -> disjoint_addr_list a2 (ocontext_addr Γ2)
                             -> OValid (ORule ls Cut (⊢app Γ1 Γ2) [d1;d2])
  | V_Ex d F G Γ1 Γ2 ls :
@@ -279,56 +327,56 @@ Inductive OValid : oderivation -> Prop :=
  
  | V_Bot' d Γ ls a: OValid d
                                 ->  OClaim d (⊢Γ) 
-                                -> Backedges d ( (1, ⊢{⊥, a}::Γ) :: lift ls)
+                                -> Backedges d ( (0, ⊢{⊥, a}::Γ) :: lift ls)
                                 -> OValid (ORule ls BotR (⊢{⊥, a}::Γ) [d])
   | V_Or_add_l' d F G Γ a ls: 
                              OValid d 
                              -> OClaim d (⊢{F,l::a}::Γ) 
-                             -> Backedges d ( (1, ⊢{ F⊕G, a }::Γ) :: lift ls)
+                             -> Backedges d ( (0, ⊢{ F⊕G, a }::Γ) :: lift ls)
                              -> OValid (ORule ls Or_add_l (⊢{ F⊕G, a }::Γ) [d])
  | V_Or_add_r' d F G Γ a ls: 
                              OValid d 
                              -> OClaim d (⊢{G,r::a}::Γ) 
-                             -> Backedges d ( (1, ⊢{ F⊕G, a }::Γ) :: lift ls)
+                             -> Backedges d ( (0, ⊢{ F⊕G, a }::Γ) :: lift ls)
                              -> OValid (ORule ls Or_add_l (⊢{ F⊕G, a }::Γ) [d])
  | V_Or_mult' d F G Γ a ls :
                             OValid d
                             -> OClaim d (⊢{ F, l::a } :: { G, r::a } :: Γ) 
-                            -> Backedges d ( (1, ⊢{ F#G, a }::Γ) :: lift ls)
+                            -> Backedges d ( (0, ⊢{ F#G, a }::Γ) :: lift ls)
                             -> OValid (ORule ls Or_mult (⊢ { F#G, a}::Γ) [d])
  | V_And_add' d1 d2 F G Γ a ls :
                             OValid d1 -> OValid d2 
                             -> OClaim d1 (⊢ { F, l::a }::Γ) -> OClaim d2 (⊢ { G, r::a }::Γ) 
-                            -> Backedges d1 ( (1, ⊢{ F&G, a }::Γ) :: lift ls)
-                            -> Backedges d2 ( (1, ⊢{ F&G, a }::Γ) :: lift ls)
+                            -> Backedges d1 ( (0, ⊢{ F&G, a }::Γ) :: lift ls)
+                            -> Backedges d2 ( (0, ⊢{ F&G, a }::Γ) :: lift ls)
                             -> OValid (ORule ls And_add (⊢ { F&G, a } :: Γ) [d1;d2])
  | V_And_mult' d1 d2 F G Γ1 Γ2 a ls :
                             OValid d1 -> OValid d2 
                             -> OClaim d1 (⊢ { F, l::a } :: Γ1) -> OClaim d2 (⊢ { G, r::a } :: Γ2) 
-                            -> Backedges d1 ( (1, ⊢{ F⊗G, a }::(app Γ1 Γ2)) :: lift ls)
-                            -> Backedges d2 ( (1, ⊢{ F⊗G, a }::(app Γ1 Γ2)) :: lift ls)
+                            -> Backedges d1 ( (0, ⊢{ F⊗G, a }::(app Γ1 Γ2)) :: lift ls)
+                            -> Backedges d2 ( (0, ⊢{ F⊗G, a }::(app Γ1 Γ2)) :: lift ls)
                             -> OValid (ORule ls And_mult (⊢ { F⊗G, a } :: (app Γ1 Γ2)) [d1;d2])
  | V_Cut' d1 d2 A Γ1 Γ2 ls a1 a2 :
                             OValid d1 -> OValid d2 
-                             -> OClaim d1 (⊢ { dual A, a1}::Γ1) -> OClaim d2 (⊢ { A, a2 }::Γ2) 
+                             -> OClaim d1 (⊢ { A, a1}::Γ1) -> OClaim d2 (⊢ { dual A, a2 }::Γ2) 
                              -> disjoint_addr_list a1 (ocontext_addr Γ1) -> disjoint_addr_list a2 (ocontext_addr Γ2)
-                             -> Backedges d1 ( (1, ⊢app Γ1 Γ2) :: lift ls)
-                            -> Backedges d2 ( (1, ⊢app Γ1 Γ2) :: lift ls)
+                             -> Backedges d1 ( (0, ⊢app Γ1 Γ2) :: lift ls) 
+                            -> Backedges d2 ( (0, ⊢app Γ1 Γ2) :: lift ls)
                              -> OValid (ORule ls Cut (⊢app Γ1 Γ2) [d1;d2])
  | V_Ex' d F G Γ1 Γ2 ls :
                             OValid d 
                             -> OClaim d (⊢ app Γ1 (G::F::Γ2)) 
-                            -> Backedges d ( (1, ⊢app Γ1 (F::G::Γ2)) :: lift ls)
+                            -> Backedges d ( (0, ⊢app Γ1 (F::G::Γ2)) :: lift ls)
                             -> OValid (ORule ls Ex (⊢app Γ1 (F::G::Γ2)) [d])
  | V_Mu' d F Γ ls a :
                            OValid d 
                            -> OClaim d (⊢ { F[[ %0 := µ F ]], i::a }::Γ)
-                           -> Backedges d ( (1, ⊢ { (µ F), a }::Γ) :: lift ls)
+                           -> Backedges d ( (0, ⊢ { (µ F), a }::Γ) :: lift ls)
                            -> OValid (ORule ls Mu (⊢ { (µ F), a }::Γ) [d])
  | V_Nu' d F Γ ls a :
                            OValid d 
                            -> OClaim d (⊢ { F[[ %0 := ν F ]], i::a }::Γ)
-                           -> Backedges d ( (1, ⊢ { (ν F), a }::Γ) :: lift ls)
+                           -> Backedges d ( (0, ⊢ { (ν F), a }::Γ) :: lift ls)
                            -> OValid (ORule ls Mu (⊢ { (ν F), a }::Γ) [d])
  
  (** FINALLY, THE BACK-EDGE RULE **)
@@ -380,6 +428,8 @@ Fixpoint print_list_oseq (ls:list (nat*osequent)) :=
   | [] => ""
   | (n, s)::ls => (print_oseq s)
   end.
+
+Local Open Scope string_scope.
 
 Fixpoint print_oderiv_list (d:oderivation): list string :=
   let '(ORule ls R s ds) := d in
@@ -438,9 +488,102 @@ Proof.
   repeat constructor. apply (R_Ax _ (// "A") [l] [r]); intuition.
 Qed.
 
+Ltac break :=
+ match goal with
+ | H : match _ with true => _ | false => _ end = true |- _ =>
+   rewrite !lazy_andb_iff in H
+ | H : match oclaim ?x with _ => _ end = true |- _ =>
+   destruct x; simpl in H; try easy; break
+ | H : match map _ ?x with _ => _ end = true |- _ =>
+   destruct x; simpl in H; try easy; break
+ | H : match ?x with _ => _ end = true |- _ =>
+   destruct x; simpl in H; try easy; break
+ | _ => idtac
+ end.
+ 
+Ltac mytac :=
+ cbn in *;
+  break;
+ rewrite ?andb_true_r, ?andb_true_iff, ?lazy_andb_iff in *;
+ repeat match goal with H : _ /\ _ |- _ => destruct H end;
+ repeat match goal with IH : Forall _ _  |- _ => inversion_clear IH end;
+ rewrite ?@Utils.eqb_eq in * by auto with typeclass_instances.
+
+Ltac rewr :=
+ unfold OClaim, BClosed in *;
+ match goal with
+ | H: _ = _ |- _ => rewrite H in *; clear H; rewr
+ | _ => rewrite ?eqb_refl
+ end.
+ 
+Local Open Scope eqb_scope.
+
 Theorem ovalid_deriv_is_OValid: forall (d:oderivation), 
-  OValid d <-> (ovalid_deriv d = true).
+  ovalid_deriv d = true <-> OValid d.
+Proof.
+  split.
+ - induction d as [ls r s ds IH] using oderivation_ind'.
+   cbn - [ovalid_deriv_step]. rewrite lazy_andb_iff. intros (H,H').
+   assert (IH' : Forall (fun d => OValid d) ds).
+   { rewrite Forall_forall in *. rewrite forallb_forall in *. auto. }
+   clear IH H'.
+   cbn in *; break.
+   + destruct o; destruct o0; cbn in H; simpl in H; apply Utils.eqb_eq in H;
+      destruct F; try(subst; eapply V_Ax; intuition; discriminate H).
+      ++ subst; apply (V_Ax_Var _ v); simpl; rewrite Utils.eqb_refl;
+           omega.
+      ++ apply (V_Ax _ (Op o F1 F2) _ a a0).
+        +++ apply op_dual.
+        +++ left; trivial.
+        +++ subst; right; left; trivial.
+     ++ apply (V_Ax _ (Quant q F) _ a a0).
+       +++ apply quant_dual.
+       +++ left; trivial.
+       +++ subst; right; left; trivial. 
+  + repeat destruct H. destruct (o =? (o2 ++ o5)%list) eqn:Heq.
+     ++ apply Utils.eqb_eq in Heq; apply Utils.eqb_eq in H3; subst. 
+          inversion_clear IH'; subst.  inversion_clear H3; subst. rewrite lazy_orb_iff in H0. destruct H0.
+        +++ apply lazy_andb_iff in H0. destruct H0. destruct o1. 
+               eapply (V_Cut _ _ F _ _ _ a); try eassumption; simpl; trivial;
+               rewrite disjoint_addr_list_is_disjoint_addr_listb; assumption.
+        +++ apply lazy_andb_iff in H0. destruct H0. destruct o1. 
+               eapply (V_Cut' _ _ F _ _ _ a); try eassumption; simpl; trivial;
+               try (rewrite disjoint_addr_list_is_disjoint_addr_listb; assumption);
+               apply Utils.eqb_eq; assumption.
+     ++ admit.
+  + admit.
+  + mytac; constructor; try assumption.
+  + mytac; constructor; try assumption.
+  + mytac; constructor; try assumption.
+  + mytac. rewrite Utils.eqb_eq in H5; rewrite Utils.eqb_eq in H4; subst.
+     eapply V_And_add; simpl; trivial.
+  + mytac; rewrite Utils.eqb_eq in H4; rewrite Utils.eqb_eq in H3; subst.
+    constructor; simpl; trivial.
+  + econstructor; intuition.
+  + inversion IH'; subst; constructor; try assumption; destruct H; apply Utils.eqb_eq in H; assumption.
+  + inversion IH'; subst; repeat destruct H; econstructor; try assumption;
+     simpl; destruct (F0 =? (F [[ % 0 := µ F]])) eqn:Heq.
+     -- rewrite Utils.eqb_eq in Heq; rewrite Utils.eqb_eq in H4; rewrite Utils.eqb_eq in H1; subst; trivial.
+     -- admit.
+  + inversion IH'; subst; repeat destruct H; econstructor; try assumption;
+     simpl; destruct (F0 =? (F [[ % 0 := ν F]])) eqn:Heq.
+     -- rewrite Utils.eqb_eq in Heq; rewrite Utils.eqb_eq in H4; rewrite Utils.eqb_eq in H1; subst; trivial.
+     -- admit.
+  + apply oseq_equiv_is_oseq_equivb in H. constructor; simpl. admit.
+- induction 1; simpl; rewr; auto; admit.
+Admitted.
+
+Lemma OValid_subderiv:
+  forall d1 d2, OValid d1 -> is_subderiv d2 d1 -> OValid d2.
 Proof.
 Admitted.
 
-    
+
+
+
+
+
+
+
+
+
